src/SDK/AlgorithmSuite.dfy
@@ -1,30 +1,27 @@
-include "../Crypto/All.dfy"
-include "../Crypto/Cipher.dfy"
-include "../Crypto/Digests.dfy"
-include "../Crypto/Signature.dfy"
+//include "../Crypto/All.dfy"
+//include "../Crypto/Cipher.dfy"
+//include "../Crypto/Digests.dfy"
+//include "../Crypto/Signature.dfy"
 include "../StandardLibrary/StandardLibrary.dfy"
 
 module AlgorithmSuite {
-
-  import opened Cipher
-  import Digests
-  import S = Signature
-  import opened StandardLibrary
+  import StandardLibrary
   import opened UInt = StandardLibrary.UInt
 
   const validIDs: set<uint16> := {0x0378, 0x0346, 0x0214, 0x0178, 0x0146, 0x0114, 0x0078, 0x0046, 0x0014};
 
   newtype ID = x | x in validIDs witness 0x0014
-  const AES_256_GCM_IV12_AUTH16_KDSHA384_SIGEC384 : ID := 0x0378
-  const AES_192_GCM_IV12_AUTH16_KDSHA384_SIGEC384 : ID := 0x0346
-  const AES_128_GCM_IV12_AUTH16_KDSHA256_SIGEC256 : ID := 0x0214
-  const AES_256_GCM_IV12_AUTH16_KDSHA256_SIGNONE  : ID := 0x0178
-  const AES_192_GCM_IV12_AUTH16_KDSHA256_SIGNONE  : ID := 0x0146
-  const AES_128_GCM_IV12_AUTH16_KDSHA256_SIGNONE  : ID := 0x0114
-  const AES_256_GCM_IV12_AUTH16_KDNONE_SIGNONE    : ID := 0x0078
-  const AES_192_GCM_IV12_AUTH16_KDNONE_SIGNONE    : ID := 0x0046
-  const AES_128_GCM_IV12_AUTH16_KDNONE_SIGNONE    : ID := 0x0014
+  const AES_256_GCM_IV12_TAG16_HKDF_SHA384_ECDSA_P384: ID := 0x0378
+  const AES_192_GCM_IV12_TAG16_HKDF_SHA384_ECDSA_P384: ID := 0x0346
+  const AES_128_GCM_IV12_TAG16_HKDF_SHA256_ECDSA_PZ256: ID := 0x0214
+  const AES_256_GCM_IV12_TAG16_HKDF_SHA256_SIGNONE: ID := 0x0178
+  const AES_192_GCM_IV12_TAG16_HKDF_SHA256_SIGNONE: ID := 0x0146
+  const AES_128_GCM_IV12_TAG16_HKDF_SHA256_SIGNONE: ID := 0x0114
+  const AES_256_GCM_IV12_TAG16_KDFNONE_SIGNONE: ID := 0x0078
+  const AES_192_GCM_IV12_TAG16_KDFNONE_SIGNONE: ID := 0x0046
+  const AES_128_GCM_IV12_TAG16_KDFNONE_SIGNONE: ID := 0x0014
 
+  /*
   datatype AlgSuite = AlgSuite(params : Cipher.CipherParams, hkdf : Digests.HMAC_ALGORITHM, sign : Option<S.ECDSAParams>)
 
   const Suite := map [
@@ -39,7 +36,6 @@ module AlgorithmSuite {
     AES_128_GCM_IV12_AUTH16_KDNONE_SIGNONE    := AlgSuite(CipherParams(AES128, 16, 12), Digests.HmacNOSHA,  None)
   ]
 
-
   function method input_key_length(x : ID) : nat {
       KeyLengthOfCipher(Suite[x].params)
   }
@@ -47,6 +43,6 @@ module AlgorithmSuite {
   function method signature_type_of_id(x : ID) : Option<S.ECDSAParams> {
     Suite[x].sign
   }
-  
+  */
 
 }
