src/StandardLibrary/StandardLibrary.dfy
@@ -9,7 +9,7 @@ module {:extern "STL"} StandardLibrary {
 
   datatype Error = IOError(msg: string) | DeserializationError(msg: string) | SerializationError(msg: string) | Error(msg : string)
 
-  datatype {:extern} Result<T> = Ok(get : T) | Err(err : string)
+  datatype {:extern} Result<T> = Success(value : T) | Failure(error : string)
 
   function Fill<T>(value: T, n: nat): seq<T>
     ensures |Fill(value, n)| == n
@@ -253,6 +253,7 @@ module {:extern "STL"} StandardLibrary {
   function method MapSeq<S, T>(s: seq<S>, f: S ~> T): seq<T>
     requires forall i :: 0 <= i < |s| ==> f.requires(s[i])
     reads set i,o | 0 <= i < |s| && o in f.reads(s[i]) :: o
+    decreases |s|
   {
       if s == []
       then []
@@ -327,11 +328,9 @@ module {:extern "STL"} StandardLibrary {
                   then false
                   else true // i+1 == a.Length && i+1 == b.Length, i.e. a == b
   }
-  
 
   lemma {:axiom} eq_multiset_eq_len<T> (s : seq<T>, s' : seq<T>)
       requires multiset(s) == multiset(s')
       ensures |s| == |s'| 
 
->>>>>>> d86c7da4676e9cfc8609dd5cb492177e18867845
 }
